WordRangeOpt Evaluability for AST bounds-checking

src/Assembly/BoundedType.v
@@ -1,377 +1,82 @@
 Require Import Bedrock.Word Bedrock.Nomega.
 Require Import NPeano NArith PArith Ndigits ZArith Znat ZArith_dec Ndec.
-Require Import List Listize Basics Bool Nsatz.
+Require Import List Listize Basics Bool Nsatz Sumbool Datatypes.
 Require Import Crypto.ModularArithmetic.ModularBaseSystemOpt.
-Require Import QhasmUtil WordizeUtil Bounds.
+Require Import QhasmUtil WordizeUtil Bounds Reflective.
 
 Import ListNotations.
 
-Section BoundedZ.
-
-  Section Trans4.
-    Definition min4 (a b c d: Z) :=
-      Z.min 0 (Z.min (Z.min a b) (Z.min c d)).
-
-    Definition max4 (a b c d: Z) :=
-      Z.max 0 (Z.max (Z.max a b) (Z.max c d)).
-
-    Ltac trans4min_tac := intros; unfold min4;
-      repeat match goal with
-      | [|- context[(Z.min ?x0 ?x1)%Z]] => is_var x1;
-        let A := fresh in let B := fresh in
-        destruct (Zmin_spec x0 x1)%Z as [A|A];
-        destruct A as [A B]; 
-        rewrite B; clear B
-      end; nomega.
-
-    Lemma trans4min_0: forall (x a b c d: Z),
-      (0 <= x)%Z -> (min4 a b c d <= x)%Z.
-    Proof. trans4min_tac. Qed.
-
-    Lemma trans4min_a: forall (x a b c d: Z),
-      (a <= x)%Z -> (min4 a b c d <= x)%Z.
-    Proof. trans4min_tac. Qed.
-
-    Lemma trans4min_b: forall (x a b c d: Z),
-      (b <= x)%Z -> (min4 a b c d <= x)%Z.
-    Proof. trans4min_tac. Qed.
-
-    Lemma trans4min_c: forall (x a b c d: Z),
-      (c <= x)%Z -> (min4 a b c d <= x)%Z.
-    Proof. trans4min_tac. Qed.
-
-    Lemma trans4min_d: forall (x a b c d: Z),
-      (d <= x)%Z -> (min4 a b c d <= x)%Z.
-    Proof. trans4min_tac. Qed.
-
-    Ltac trans4max_tac := intros; unfold max4;
-      repeat match goal with
-      | [|- context[(Z.max ?x0 ?x1)%Z]] => is_var x1;
-        let A := fresh in let B := fresh in
-        destruct (Zmax_spec x0 x1)%Z as [A|A];
-        destruct A as [A B]; 
-        rewrite B; clear B
-      end; try nomega.
-
-    Lemma trans4max_0: forall (x a b c d: Z),
-      (x <= 0)%Z -> (x <= max4 a b c d)%Z.
-    Proof. trans4max_tac. Qed.
-
-    Lemma trans4max_a: forall (x a b c d: Z),
-      (x <= a)%Z -> (x <= max4 a b c d)%Z.
-    Proof. trans4max_tac. Qed.
-
-    Lemma trans4max_b: forall (x a b c d: Z),
-      (x <= b)%Z -> (x <= max4 a b c d)%Z.
-    Proof. trans4max_tac. Qed.
-
-    Lemma trans4max_c: forall (x a b c d: Z),
-      (x <= c)%Z -> (x <= max4 a b c d)%Z.
-    Proof. trans4max_tac. Qed.
-
-    Lemma trans4max_d: forall (x a b c d: Z),
-      (x <= d)%Z -> (x <= max4 a b c d)%Z.
-    Proof. trans4max_tac. Qed.
-  End Trans4.
-
-  Section BoundedMul.
-    Lemma bZMul_min: forall (x0 low0 high0 x1 low1 high1: Z),
-      (low0 <= x0)%Z -> (x0 <= high0)%Z ->
-      (low1 <= x1)%Z -> (x1 <= high1)%Z ->
-      (min4 (low0 * low1) (low0 * high1)
-            (high0 * low1) (high0 * high1) <= x0 * x1)%Z.
-    Proof.
-      intros x0 low0 high0 x1 low1 high1
-        Hlow0 Hhigh0 Hlow1 Hhigh1.
-      destruct (Z_le_dec 0 x0), (Z_le_dec 0 x1).
-
-      - apply trans4min_0.
-        replace 0%Z with (0*0)%Z by nomega.
-        apply Z.mul_le_mono_nonneg; nomega.
-
-      - apply trans4min_c.
-        transitivity (x0 * low1)%Z.
-
-        + apply Z.mul_le_mono_nonpos_r; try nomega.
-        + apply Z.mul_le_mono_nonneg_l; try nomega.
-
-      - apply trans4min_b.
-        transitivity (x0 * high1)%Z.
-
-        + apply Z.mul_le_mono_nonneg_r; try nomega.
-        + apply Z.mul_le_mono_nonpos_l; try nomega.
-
-      - apply trans4min_0.
-        replace 0%Z with (0*0)%Z by nomega.
-        apply Z.mul_le_mono_nonpos; try nomega.
-    Qed.
-
-    Lemma bZMul_max: forall (x0 low0 high0 x1 low1 high1: Z),
-      (low0 <= x0)%Z -> (x0 <= high0)%Z ->
-      (low1 <= x1)%Z -> (x1 <= high1)%Z ->
-      (x0 * x1 <=
-      max4 (low0 * low1) (low0 * high1)
-           (high0 * low1) (high0 * high1))%Z.
-    Proof.
-      intros x0 low0 high0 x1 low1 high1
-        Hlow0 Hhigh0 Hlow1 Hhigh1.
-      destruct (Z_le_dec 0 x0), (Z_le_dec 0 x1).
-
-      - apply trans4max_d.
-        apply Z.mul_le_mono_nonneg; nomega.
-
-      - apply trans4max_0.
-        replace 0%Z with (0*0)%Z by nomega.
-        transitivity (x0 * 0)%Z.
-
-        + apply Z.mul_le_mono_nonneg_l; try nomega.
-        + apply Z.mul_le_mono_nonpos_r; try nomega.
-
-      - apply trans4max_0.
-        replace 0%Z with (0*0)%Z by nomega.
-        transitivity (x0 * 0)%Z.
-
-        + apply Z.mul_le_mono_nonpos_l; try nomega.
-        + apply Z.mul_le_mono_nonneg_r; try nomega.
-
-      - apply trans4max_a.
-        apply Z.mul_le_mono_nonpos; try nomega.
-    Qed.
-  End BoundedMul.
-
-  Inductive BoundedZ :=
-    | boundedZ: forall (x low high: Z),
-      (low <= x)%Z -> (x <= high)%Z -> BoundedZ.
-
-  Definition bprojZ (x: BoundedZ) :=
-    match x with
-    | boundedZ x0 low0 high0 plow0 phigh0 => x0
-    end.
-
-  Definition bZAdd (a b: BoundedZ): BoundedZ.
-    refine match a with
-    | boundedZ x0 low0 high0 plow0 phigh0 =>
-      match b with
-      | boundedZ x1 low1 high1 plow1 phigh1 =>
-        boundedZ (x0 + x1) (low0 + low1) (high0 + high1) _ _
-      end
-    end; abstract nomega.
-  Defined.
-
-  Definition bZSub (a b: BoundedZ): BoundedZ.
-    refine match a with
-    | boundedZ x0 low0 high0 plow0 phigh0 =>
-      match b with
-      | boundedZ x1 low1 high1 plow1 phigh1 =>
-        boundedZ (x0 - x1) (low0 - high1) (high0 - low1) _ _
-      end
-    end; abstract nomega.
-  Defined.
-
-  Definition bZMul (a b: BoundedZ): BoundedZ.
-    refine match a with
-    | boundedZ x0 low0 high0 plow0 phigh0 =>
-      match b with
-      | boundedZ x1 low1 high1 plow1 phigh1 =>
-        boundedZ (x0 * x1)
-          (min4 (low0 * low1) (low0 * high1)
-                (high0 * low1) (high0 * high1))
-          (max4 (low0 * low1) (low0 * high1)
-                (high0 * low1) (high0 * high1))
-          _ _
-      end
-    end; try apply bZMul_min; try apply bZMul_max; try assumption.
-  Defined.
-
-  Definition bZShiftr (a: BoundedZ) (k: nat): BoundedZ.
-    assert (forall k, 2 ^ (Z.of_nat k) > 0)%Z as H by abstract (
-      intro m;
-      rewrite <- two_p_equiv;
-      apply two_p_gt_ZERO;
-      induction m; try reflexivity;
-      rewrite Nat2Z.inj_succ;
-      nomega).
-
-    refine match a with
-    | boundedZ x low high plow phigh =>
-      boundedZ (Z.shiftr x (Z.of_nat k))
-               (Z.shiftr low (Z.of_nat k))
-               (Z.succ (Z.shiftr high (Z.of_nat k))) _ _
-    end.
-
-    - abstract (
-        repeat rewrite Z.shiftr_div_pow2;
-        try apply Nat2Z.is_nonneg;
-        apply Z_div_le; try assumption;
-        try apply H).
-
-    - abstract (
-        apply Z.lt_succ_r;
-        repeat rewrite Z.shiftr_div_pow2;
-        try apply Nat2Z.is_nonneg;
-        apply Z.lt_lt_succ_r;
-        apply Z.lt_succ_r;
-        apply Z_div_le;
-        try apply H;
-        try assumption).
-  Qed.
-
-  Definition bZMask (a: BoundedZ) (k: nat): BoundedZ.
-    assert (0 < 2 ^ Z.of_nat k)%Z as Hk by (
-      induction k;
-      try abstract (vm_compute; reflexivity);
-      rewrite Nat2Z.inj_succ;
-      rewrite <- two_p_equiv;
-      apply Z.gt_lt;
-      apply two_p_gt_ZERO;
-      apply Z.le_le_succ_r;
-      apply Nat2Z.is_nonneg).
-
-    refine match a with
-    | boundedZ x low high plow phigh =>
-      boundedZ (Z.land x (Z.ones (Z.of_nat k)))
-               (Z.of_N 0%N)
-               (Z.of_N (Npow2 k)) _ _
-    end.
-
-    - repeat rewrite Z.land_ones;
-        try apply Nat2Z.is_nonneg.
-
-      abstract (
-        apply (Z.mod_pos_bound x) in Hk; destruct Hk;
-        induction k; simpl in *; assumption).
-
-    - repeat rewrite Z.land_ones;
-        try apply Nat2Z.is_nonneg.
-
-      abstract (
-        rewrite Npow2_N;
-        rewrite N2Z.inj_pow; simpl;
-        apply (Z.mod_pos_bound x) in Hk; destruct Hk;
-        apply Z.lt_le_incl;
-        induction k; simpl in *; assumption).
-  Qed.
-End BoundedZ.
-
-Section BoundedN.
-
-  Inductive BoundedN :=
-    | boundedN: forall (x low high: N),
-      (low <= x)%N -> (x < high)%N -> BoundedN.
-
-  Definition bprojN (x: BoundedN) :=
-    match x with
-    | boundedN x0 low0 high0 plow0 phigh0 => x0
-    end.
-
-  Definition bNAdd (a b: BoundedN): BoundedN.
-    refine match a with
-    | boundedN x0 low0 high0 plow0 phigh0 =>
-      match b with
-      | boundedN x1 low1 high1 plow1 phigh1 =>
-        boundedN (x0 + x1) (low0 + low1) (high0 + high1) _ _
-      end
-    end.
-
-    - abstract (apply N.add_le_mono; assumption).
-    - abstract nomega.
-  Defined.
-
-  Definition bNSub (a b: BoundedN): BoundedN.
-    refine match a with
-    | boundedN x0 low0 high0 plow0 phigh0 =>
-      match b with
-      | boundedN x1 low1 high1 plow1 phigh1 =>
-        boundedN (x0 - x1) (low0 - high1) (N.succ (high0 - low1)) _ _
-      end
-    end.
-
-    - transitivity (x0 - high1)%N.
-
-      + apply N.sub_le_mono_r; assumption.
-      + apply N.sub_le_mono_l; apply N.lt_le_incl; assumption.
-
-    - apply N.lt_succ_r; transitivity (high0 - x1)%N.
-
-      + apply N.sub_le_mono_r; apply N.lt_le_incl; assumption.
-      + apply N.sub_le_mono_l; assumption.
-
-  Defined.
-
-  Definition bNMul (a b: BoundedN): BoundedN.
-    refine match a with
-    | boundedN x0 low0 high0 plow0 phigh0 =>
-      match b with
-      | boundedN x1 low1 high1 plow1 phigh1 =>
-        boundedN (x0 * x1)%N (low0 * low1)%N (high0 * high1)%N _ _
-      end
-    end; abstract (
-      try apply N.mul_le_mono_nonneg;
-      try apply N.mul_lt_mono_nonneg;
-        try assumption;
-        try apply N_ge_0).
-  Qed.
-
-  Definition bNShiftr (a: BoundedN) (k: nat): BoundedN.
-    assert (forall k, 2 ^ (N.of_nat k) > 0)%N as H by abstract (
-      intros;
-      rewrite <- Npow2_N;
-      apply N.lt_gt;
-      apply Npow2_gt0).
-
-    refine match a with
-    | boundedN x low high plow phigh =>
-      boundedN (N.shiftr x (N.of_nat k))
-               (N.shiftr low (N.of_nat k))
-               (N.succ (N.shiftr high (N.of_nat k))) _ _
-    end.
-
-    - abstract (
-        repeat rewrite N.shiftr_div_pow2;
-        apply N.div_le_mono; try assumption;
-        pose proof (H k) as H0;
-        induction ((2 ^ N.of_nat k)%N);
-        inversion H0; intuition).
-
-    - abstract (
-        apply N.lt_succ_r;
-        repeat rewrite N.shiftr_div_pow2;
-        apply N.div_le_mono;
-        try apply N.lt_le_incl;
-        pose proof (H k) as H0;
-        induction ((2 ^ N.of_nat k)%N);
-        inversion H0; intuition).
-  Defined.
-
-  Definition bNMask (a: BoundedN) (k: nat): BoundedN.
-    assert (forall k, 0 < 2 ^ (N.of_nat k))%N as H by abstract (
-      intros;
-      rewrite <- Npow2_N;
-      apply Npow2_gt0).
-
-    refine match a with
-    | boundedN x low high plow phigh =>
-      boundedN (N.land x (N.ones (N.of_nat k)))
-               0%N
-               (Npow2 k) _ _
-    end.
-
-    - repeat rewrite N.land_ones;
-        apply N_ge_0.
-
-    - repeat rewrite N.land_ones.
-
-      abstract (
-        rewrite Npow2_N;
-        pose proof (N.mod_bound_pos x (2 ^ N.of_nat k)%N (N_ge_0 _) (H k))
-          as H0; destruct H0;
-        assumption).
-  Defined.
-
-End BoundedN.
-
-Section BoundedWord.
+Section Z.
+  Instance ZEvaluable : Evaluable Z := {
+    ezero := 0%Z;
+
+    (* Conversions *)
+    toT := Z.of_nat;
+    fromT := Z.to_nat;
+
+    (* Operations *)
+    eadd := Z.add;
+    esub := Z.sub;
+    emul := Z.mul;
+    eshiftr := fun x k => Z.shiftr x (Z.of_nat k);
+    emask := fun x k => Z.land x (Z.ones (Z.of_nat k));
+
+    (* Comparisons *)
+    eltb := Z.ltb;
+    eeqb := Z.eqb;
+  }.
+End Z.
+
+Section Word.
   Context {n: nat}.
+
+  Instance WordEvaluable : Evaluable (word n) := {
+    ezero := wzero n;
+
+    (* Conversions *)
+    toT := natToWord n;
+    fromT := @wordToNat n;
+
+    (* Operations *)
+    eadd := @wplus n;
+    esub := @wminus n;
+    emul := @wmult n;
+    eshiftr := @shiftr n;
+    emask := fun x k => @mask n k x;
+
+    (* Comparisons *)
+    eltb := fun x y => N.ltb (wordToN x) (wordToN y);
+    eeqb := fun x y => proj1_sig (bool_of_sumbool (@weq n x y))
+  }.
+End Word.
+
+Section RangeUpdate.
+  Context {n: nat}.
+
+  Inductive Range T := | range: forall (low high: T), Range T.
+
+  Definition validBinaryWordOp
+        (rangeF: Range N -> Range N -> option (Range N))
+        (wordF: word n -> word n -> word n): Prop :=
+    forall (low0 high0 low1 high1: N) (x y: word n),
+      (low0 <= wordToN x < high0)%N
+    -> (low1 <= wordToN y < high1)%N
+    -> match rangeF (range N low0 high0) (range N low1 high1) with
+      | Some (range low2 high2) =>
+        (low2 <= @wordToN n (wordF x y) < high2)%N
+      | _ => True 
+      end.
+
+  Definition validNatWordOp
+        (rangeF: Range N -> nat -> option (Range N))
+        (wordF: word n -> nat -> word n): Prop :=
+    forall (low0 high0: N) (k: nat) (x: word n),
+      (low0 <= wordToN x < high0)%N
+    -> match rangeF (range N low0 high0) k with
+      | Some (range low2 high2) =>
+        (low2 <= @wordToN n (wordF x k) < high2)%N
+      | _ => True 
+      end.
 
   Section BoundedSub.
     Lemma NToWord_Npow2: wzero n = NToWord n (Npow2 n).
@@ -597,30 +302,22 @@ Section BoundedWord.
     Qed.
   End BoundedSub.
 
-  Inductive BoundedWord :=
-    | boundedWord: forall (x: word n) (low high: N) (overflowed: bool),
-      (low <= wordToN x)%N -> (wordToN x < high)%N -> BoundedWord.
+  Lemma range_add_valid :
+    validBinaryWordOp
+      (fun range0 range1 =>
+         match (range0, range1) with
+         | (range low0 high0, range low1 high1) =>
+           if (overflows n (high0 + high1))
+           then None
+           else Some (range N (low0 + low1) (high0 + high1))
+         end)%N
+      (@wplus n).
+  Proof.
+    unfold validBinaryWordOp; intros until y; intros H0 H1.
+    destruct H0 as [H0a H0b].
+    destruct H1 as [H1a H1b].
 
-  Definition bprojW (x: BoundedWord) :=
-    match x with
-    | boundedWord x0 _ _ _ _ _ => x0
-    end.
-
-  Definition bWAdd (a b: BoundedWord): BoundedWord.
-    refine match a with
-    | boundedWord x0 low0 high0 o0 plow0 phigh0 =>
-      match b with
-      | boundedWord x1 low1 high1 o1 plow1 phigh1 =>
-        if (overflows n (high0 + high1))
-        then boundedWord (x0 ^+ x1) 0%N (high0 + high1) true _ _
-        else boundedWord (x0 ^+ x1) (low0 + low1) (high0 + high1) (orb o0 o1) _ _
-      end
-    end; try abstract (
-      apply (N.le_lt_trans _ (wordToN x0 + wordToN x1)%N _);
-        try apply plus_le;
-        abstract nomega).
-
-    - apply N_ge_0.
+    destruct (overflows n (high0 + high1))%N; split.
 
     - erewrite <- wordize_plus';
         try eassumption;
@@ -628,50 +325,57 @@ Section BoundedWord.
 
       + apply N.add_le_mono; assumption.
 
-      + abstract (apply N.lt_le_incl; nomega).
+      + apply N.lt_le_incl; nomega.
+
+    - apply (N.le_lt_trans _ (wordToN x + wordToN y)%N _);
+        try apply plus_le.
+      nomega.
   Qed.
 
-  Definition bWSub (a b: BoundedWord): BoundedWord.
-    refine match a with
-    | boundedWord x0 low0 high0 o0 plow0 phigh0 =>
-      match b with
-      | boundedWord x1 low1 high1 o1 plow1 phigh1 =>
-        let upper_bound :=
-          if (Nge_dec high0 (Npow2 n))
-          then Npow2 n
-          else if (Nge_dec high1 (Npow2 n))
-               then Npow2 n
-               else (N.succ (high0 + Npow2 n - low1)) in
+  Lemma range_sub_valid :
+    validBinaryWordOp
+      (fun range0 range1 =>
+         match (range0, range1) with
+         | (range low0 high0, range low1 high1) =>
+           if (Nge_dec low0 high1)
+           then Some (range N (low0 - high1)%N
+              (if (Nge_dec high0 (Npow2 n)) then Npow2 n else
+               if (Nge_dec high1 (Npow2 n)) then Npow2 n else
+               N.succ (high0 + Npow2 n - low1))%N)
+           else None
+         end)
+      (@wminus n).
+  Proof.
+    unfold validBinaryWordOp; intros until y; intros H0 H1.
+    destruct H0 as [H0a H0b].
+    destruct H1 as [H1a H1b].
 
-        if (Nge_dec low0 high1)
-        then boundedWord (x0 ^- x1) (low0 - high1)%N upper_bound (orb o0 o1) _ _
-        else boundedWord (x0 ^- x1) 0%N upper_bound true _ _
-      end
-    end; abstract (unfold upper_bound; try apply N_ge_0;
-      destruct (Nge_dec high0 (Npow2 n)), (Nge_dec high1 (Npow2 n));
+    destruct (Nge_dec high0 (Npow2 n)),
+             (Nge_dec high1 (Npow2 n)),
+             (Nge_dec low0 high1); split;
       repeat match goal with
       | [|- (_ - ?x <= wordToN _)%N] => apply bWSub_lem0
       | [|- (wordToN _ < N.succ (?x + _ - _))%N] => apply bWSub_lem1
       | [|- (wordToN _ < Npow2 _)%N] => apply word_size_bound
       | [|- (0 <= _)%N] => apply N_ge_0
-      end; assumption).
+      end; assumption.
   Qed.
 
-  Definition bWMul (a b: BoundedWord): BoundedWord.
-    refine match a with
-    | boundedWord x0 low0 high0 o0 plow0 phigh0 =>
-      match b with
-      | boundedWord x1 low1 high1 o1 plow1 phigh1 =>
-        if (overflows n (high0 * high1))
-        then boundedWord (x0 ^* x1)%N 0%N (high0 * high1)%N true _ _
-        else boundedWord (x0 ^* x1)%N (low0 * low1)%N (high0 * high1)%N (orb o0 o1) _ _
-      end
-    end.
+  Lemma range_mul_valid :
+    validBinaryWordOp
+      (fun range0 range1 =>
+         match (range0, range1) with
+         | (range low0 high0, range low1 high1) =>
+           if (overflows n (high0 * high1)) then None else
+           Some (range N (low0 * low1) (high0 * high1))%N
+          end)
+      (@wmult n).
+  Proof.
+    unfold validBinaryWordOp; intros until y; intros H0 H1.
+    destruct H0 as [H0a H0b].
+    destruct H1 as [H1a H1b].
 
-    - apply N_ge_0.
-
-    - apply (N.le_lt_trans _ (wordToN x0 * wordToN x1)%N _); [apply mult_le|].
-      apply N.mul_lt_mono; assumption.
+    destruct (overflows n (high0 * high1))%N; split.
 
     - rewrite <- wordize_mult.
 
@@ -680,53 +384,145 @@ Section BoundedWord.
       + transitivity (high0 * high1)%N; [|assumption].
         apply N.mul_lt_mono; assumption.
 
-    - apply (N.le_lt_trans _ (wordToN x0 * wordToN x1)%N _); [apply mult_le|].
+    - apply (N.le_lt_trans _ (wordToN x * wordToN y)%N _); [apply mult_le|].
       apply N.mul_lt_mono; assumption.
   Qed.
 
-  Definition bWShiftr (a: BoundedWord) (k: nat): BoundedWord.
-    assert (forall k, 2 ^ (N.of_nat k) > 0)%N as H by abstract (
-      intros;
-      rewrite <- Npow2_N;
-      apply N.lt_gt;
-      apply Npow2_gt0).
+  Lemma range_shiftr_valid :
+    validNatWordOp
+      (fun range0 k =>
+         match range0 with
+         | range low high =>
+           Some (range N
+             (N.shiftr low (N.of_nat k))
+             (N.succ (N.shiftr high (N.of_nat k))))
+          end)
+      (fun x k => extend (Nat.eq_le_incl _ _ eq_refl) (shiftr x k)).
+  Proof.
+    unfold validNatWordOp; intros until x; intro H.
+    destruct H as [Ha Hb]; split.
 
-    refine match a with
-    | boundedWord x low high o plow phigh =>
-      boundedWord (extend _ (shiftr x k))
-        (N.shiftr low (N.of_nat k))
-        (N.succ (N.shiftr high (N.of_nat k))) o _ _
+    - unfold extend; rewrite wordToN_convS.
+
+      rewrite wordToN_zext.
+      rewrite <- wordize_shiftr.
+      rewrite <- Nshiftr_equiv_nat.
+      repeat rewrite N.shiftr_div_pow2.
+      apply N.div_le_mono; [|assumption].
+      induction k.
+
+      + cbv beta delta iota; intro Z; inversion Z.
+
+      + rewrite <- Npow2_N.
+        pose proof (Npow2_gt0 (S k)).
+        nomega.
+
+    - unfold extend; rewrite wordToN_convS.
+      rewrite wordToN_zext.
+      rewrite Nshiftr_equiv_nat.
+      eapply N.lt_le_trans.
+
+      + apply shiftr_bound; eassumption.
+
+      + apply N.eq_le_incl.
+        reflexivity.
+  Qed.
+
+  Lemma range_mask_valid :
+    validNatWordOp
+      (fun range0 k =>
+         match range0 with
+         | range low high =>
+           Some (range N 0%N (Npow2 k))
+          end)
+      (fun x k => mask k x).
+  Proof.
+    unfold validNatWordOp; intros until x; intro H.
+    destruct H as [Ha Hb]; split; [apply N_ge_0|].
+    apply mask_bound.
+  Qed.
+End RangeUpdate.
+
+Section WordRange.
+  Context {n: nat}.
+
+  Inductive WordRangeOpt :=
+    | someRange: forall (low high: N),
+        (low < high)%N -> (high <= Npow2 n)%N -> WordRangeOpt
+    | applyBinOp: forall rangeF wordF,
+        @validBinaryWordOp n rangeF wordF ->
+        WordRangeOpt -> WordRangeOpt -> WordRangeOpt
+    | applyNatOp: forall rangeF wordF,
+        @validNatWordOp n rangeF wordF ->
+        WordRangeOpt -> nat -> WordRangeOpt.
+
+  Fixpoint evalWordRangeOpt (r: WordRangeOpt): option (Range N) :=
+    match r with
+    | someRange low high _ _ => Some (range N low high)
+    | applyBinOp rangeF wordF _ a b =>
+      omap (evalWordRangeOpt a) (fun a' =>
+        omap (evalWordRangeOpt a) (fun b' =>
+          rangeF a' b'))
+    | applyNatOp rangeF wordF _ x k =>
+      omap (evalWordRangeOpt x) (fun x' =>
+        rangeF x' k)
     end.
 
-    - unfold extend; rewrite wordToN_convS.
+  Definition anyWord: WordRangeOpt.
+    refine (someRange 0%N (Npow2 n) _ _).
+    - apply Npow2_gt0.
+    - reflexivity.
+  Defined.
 
-      abstract (
-        rewrite wordToN_zext;
-        rewrite <- wordize_shiftr;
-        rewrite <- Nshiftr_equiv_nat;
-        repeat rewrite N.shiftr_div_pow2;
-        apply N.div_le_mono; try assumption;
-        pose proof (H k) as H0;
-        induction ((2 ^ N.of_nat k)%N);
-        inversion H0; intuition).
+  Definition getLowerBoundOpt (w: WordRangeOpt): option N :=
+    omap (evalWordRangeOpt w) (fun r =>
+      match r with | range low high => Some low end).
 
-    - unfold extend; rewrite wordToN_convS.
-      abstract (
-        rewrite wordToN_zext;
-        rewrite Nshiftr_equiv_nat;
-        eapply N.lt_le_trans;
-        try apply shiftr_bound;
-        try apply N.eq_le_incl;
-        try eassumption; reflexivity).
+  Definition getUpperBoundOpt (w: WordRangeOpt): option N :=
+    omap (evalWordRangeOpt w) (fun r =>
+      match r with | range low high => Some high end).
 
-    Unshelve.
-    reflexivity.
-  Qed.
+  Definition makeRangeOpt (low high: N): option WordRangeOpt.
+    refine (
+      match (Nge_dec low high, Nge_dec high (Npow2 n)) with
+      | (right _, right _) => Some (someRange low high _ _)
+      | _ => None
+      end); [assumption|].
 
-  Definition bWMask (a: BoundedWord) (k: nat): BoundedWord.
-    refine match a with
-    | boundedWord x low high o plow phigh =>
-      boundedWord (mask k x) 0%N (Npow2 k) o _ _
-    end; [apply N_ge_0 | apply mask_bound].
-  Qed.
-End BoundedWord.
+    apply N.lt_le_incl; assumption.
+  Defined.
+
+  Definition getOrElse {T} (d: T) (o: option T) :=
+    match o with | Some x => x | None => d end.
+
+  Instance WordRangeOptEvaluable : Evaluable WordRangeOpt := {
+    ezero := anyWord;
+
+    (* Conversions *)
+    toT := fun x => getOrElse anyWord (makeRangeOpt 0%N (N.of_nat x));
+    fromT := fun x => getOrElse (pow2 n) (option_map N.to_nat (getUpperBoundOpt x));
+
+    (* Operations *)
+    eadd := applyBinOp _ _ range_add_valid;
+    esub := applyBinOp _ _ range_sub_valid;
+    emul := applyBinOp _ _ range_mul_valid;
+    eshiftr := applyNatOp _ _ range_shiftr_valid;
+    emask := applyNatOp _ _ range_mask_valid;
+
+    (* Comparisons just test upper bounds.
+       We won't bounds-check Ite in our PHOAS formalism *)
+    eltb := fun x y =>
+      getOrElse false (
+        omap (getUpperBoundOpt x) (fun xb =>
+          omap (getUpperBoundOpt y) (fun yb =>
+            Some (N.ltb xb yb))));
+
+    eeqb := fun x y =>
+      getOrElse false (
+        omap (getUpperBoundOpt x) (fun xub =>
+          omap (getUpperBoundOpt y) (fun yub =>
+            omap (getLowerBoundOpt x) (fun xlb =>
+              omap (getLowerBoundOpt y) (fun ylb =>
+                Some (andb (N.eqb xub yub) (N.eqb xlb ylb)))))))
+  }.
+End WordRange.
